tests/lean/Avl/Specifications.lean
@@ -1,4 +1,4 @@
-import Avl.Extracted
+import Avl.Tree
 
 namespace Primitives
 
@@ -23,27 +23,27 @@ end Result
 
 end Primitives
 
-namespace avl_verification
+namespace avl
 
 @[simp]
-def Ordering.toLeanOrdering (o: avl_verification.Ordering): _root_.Ordering := match o with 
+def Ordering.toLeanOrdering (o: avl.Ordering): _root_.Ordering := match o with
 | .Less => .lt
 | .Equal => .eq
 | .Greater => .gt
 
-def Ordering.ofLeanOrdering (o: _root_.Ordering): avl_verification.Ordering := match o with
+def Ordering.ofLeanOrdering (o: _root_.Ordering): avl.Ordering := match o with
 | .lt => .Less
 | .eq => .Equal
 | .gt => .Greater
 
 @[simp]
-def Ordering.toDualOrdering (o: avl_verification.Ordering): avl_verification.Ordering := match o with 
+def Ordering.toDualOrdering (o: avl.Ordering): avl.Ordering := match o with
 | .Less => .Greater
 | .Equal => .Equal
 | .Greater => .Less
 
 @[simp]
-theorem Ordering.toLeanOrdering.injEq (x y: avl_verification.Ordering): (x.toLeanOrdering = y.toLeanOrdering) = (x = y) := by
+theorem Ordering.toLeanOrdering.injEq (x y: avl.Ordering): (x.toLeanOrdering = y.toLeanOrdering) = (x = y) := by
   apply propext
   cases x <;> cases y <;> simp
 
@@ -62,36 +62,36 @@ theorem ite_eq_gt_distrib (c : Prop) [Decidable c] (a b : Ordering) :
     ((if c then a else b) = .Greater) = if c then a = .Greater else b = .Greater := by
   by_cases c <;> simp [*]
 
-end avl_verification
+end avl
 
 namespace Specifications
 
 open Primitives
 open Result
 
-variable {T: Type} (H: outParam (avl_verification.Ord T))
+variable {T: Type} (H: outParam (avl.Ord T))
 
 @[simp]
-def _root_.Ordering.toDualOrdering (o: _root_.Ordering): _root_.Ordering := match o with 
+def _root_.Ordering.toDualOrdering (o: _root_.Ordering): _root_.Ordering := match o with
 | .lt => .gt
 | .eq => .eq
 | .gt => .lt
 
 
 @[simp]
-theorem toDualOrderingOfToLeanOrdering (o: avl_verification.Ordering): o.toDualOrdering.toLeanOrdering = o.toLeanOrdering.toDualOrdering := by
+theorem toDualOrderingOfToLeanOrdering (o: avl.Ordering): o.toDualOrdering.toLeanOrdering = o.toLeanOrdering.toDualOrdering := by
   cases o <;> simp
 
 @[simp]
-theorem toDualOrderingIdempotency (o: _root_.Ordering): o.toDualOrdering.toDualOrdering = o := by 
+theorem toDualOrderingIdempotency (o: _root_.Ordering): o.toDualOrdering.toDualOrdering = o := by
   cases o <;> simp
 
 -- TODO: reason about raw bundling vs. refined bundling.
 -- raw bundling: hypothesis with Rust extracted objects.
 -- refined bundling: lifted hypothesis with Lean native objects.
 class OrdSpec [Ord T] where
-  infallible: ∀ a b, ∃ (o: avl_verification.Ordering), H.cmp a b = .ok o ∧ compare a b = o.toLeanOrdering
-  
+  infallible: ∀ a b, ∃ (o: avl.Ordering), H.cmp a b = .ok o ∧ compare a b = o.toLeanOrdering
+
 class OrdSpecSymmetry [O: Ord T] extends OrdSpec H where
   symmetry: ∀ a b, O.compare a b = (O.opposite.compare a b).toDualOrdering
 
@@ -101,11 +101,11 @@ class OrdSpecRel [O: Ord T] (R: outParam (T -> T -> Prop)) extends OrdSpec H whe
 
 class OrdSpecLinearOrderEq [O: Ord T] extends OrdSpecSymmetry H, OrdSpecRel H Eq
 
-theorem infallible [Ord T] [OrdSpec H]: ∀ a b, ∃ o, H.cmp a b = .ok o := fun a b => by 
+theorem infallible [Ord T] [OrdSpec H]: ∀ a b, ∃ o, H.cmp a b = .ok o := fun a b => by
   obtain ⟨ o, ⟨ H, _ ⟩ ⟩ := OrdSpec.infallible a b
   exact ⟨ o, H ⟩
 
-instance: Coe (avl_verification.Ordering) (_root_.Ordering) where
+instance: Coe (avl.Ordering) (_root_.Ordering) where
   coe a := a.toLeanOrdering
 
 theorem rustCmpEq [Ord T] [O: OrdSpec H]: H.cmp a b = .ok o <-> compare a b = o.toLeanOrdering := by
@@ -116,7 +116,7 @@ theorem rustCmpEq [Ord T] [O: OrdSpec H]: H.cmp a b = .ok o <-> compare a b = o.
     simp [Hcompare, Hcmp', Hcmp]
   . intro Hcompare
     obtain ⟨ o', ⟨ Hcmp', Hcompare' ⟩ ⟩ := O.infallible a b
-    rw [Hcompare', avl_verification.Ordering.toLeanOrdering.injEq] at Hcompare
+    rw [Hcompare', avl.Ordering.toLeanOrdering.injEq] at Hcompare
     simp [Hcompare.symm, Hcmp']
 
 
@@ -125,21 +125,21 @@ theorem oppositeOfOpposite {x y: _root_.Ordering}: x.toDualOrdering = y ↔ x = 
 theorem oppositeRustOrder [Ord T] [Spec: OrdSpecSymmetry H] {a b}: H.cmp b a = .ok o ↔ H.cmp a b = .ok o.toDualOrdering := by
   rw [rustCmpEq, Spec.symmetry, compare, Ord.opposite, oppositeOfOpposite, rustCmpEq, toDualOrderingOfToLeanOrdering]
 
-theorem ltOfRustOrder 
+theorem ltOfRustOrder
   [LO: LinearOrder T]
-  [Spec: OrdSpec H]: 
+  [Spec: OrdSpec H]:
   ∀ a b, H.cmp a b = .ok .Less -> a < b := by
   intros a b
   intro Hcmp
   -- why the typeclass search doesn't work here?
   refine' (@compare_lt_iff_lt T LO).1 _
-  obtain ⟨ o, ⟨ Hcmp', Hcompare ⟩ ⟩ := Spec.infallible a b 
+  obtain ⟨ o, ⟨ Hcmp', Hcompare ⟩ ⟩ := Spec.infallible a b
   simp only [Hcmp', ok.injEq] at Hcmp
-  simp [Hcompare, Hcmp, avl_verification.Ordering.toLeanOrdering]
+  simp [Hcompare, Hcmp, avl.Ordering.toLeanOrdering]
 
-theorem gtOfRustOrder 
+theorem gtOfRustOrder
   [LinearOrder T]
-  [Spec: OrdSpecSymmetry H]: 
+  [Spec: OrdSpecSymmetry H]:
   ∀ a b, H.cmp a b = .ok .Greater -> b < a := by
   intros a b
   intro Hcmp
