tests/lean/Avl.lean
@@ -1,7 +1,5 @@
-import Avl.Extracted
--- import Avl.Insert ; TODO: the insert_loop does not exist anymore!
+import Avl.Insert
 import Avl.Find
 import Avl.Order
 import Avl.Height
 import Avl.Rotate
-import Avl.Rebalance.Complete
