tests/lean/Avl/BinarySearchTree.lean
@@ -3,14 +3,14 @@ import Avl.Tree
 namespace BST
 
 open Primitives (Result Scalar)
-open avl_verification (AVLNode Ordering)
+open avl (AVLNode Ordering)
 open Tree (AVLTree AVLNode.left AVLNode.right AVLNode.val)
 
 -- TODO: build a function to build a tree out of a left and right
 -- with automatic height computation?
 
 @[reducible]
-def AVLNode.mk' (a: T) (left: AVLTree T) (right: AVLTree T): AVLNode T := 
+def AVLNode.mk' (a: T) (left: AVLTree T) (right: AVLTree T): AVLNode T :=
   let height := 1 + max left.height right.height
   -- TODO: Scalar.ofNat would be nice...
   -- discharge the proof by bounding left & right's height all the time... ?
@@ -26,26 +26,26 @@ inductive ForallNode (p: T -> Prop): AVLTree T -> Prop
 
 theorem ForallNode.left {p: T -> Prop} {t: AVLTree T}: ForallNode p t -> ForallNode p t.left := by
   intro Hpt
-  cases Hpt with 
+  cases Hpt with
   | none => simp [AVLTree.left, ForallNode.none]
   | some a left right f_pleft f_pa f_pright => simp [AVLTree.left, f_pleft]
 
 theorem ForallNode.right {p: T -> Prop} {t: AVLTree T}: ForallNode p t -> ForallNode p t.right := by
   intro Hpt
-  cases Hpt with 
+  cases Hpt with
   | none => simp [AVLTree.right, ForallNode.none]
   | some a left right f_pleft f_pa f_pright => simp [AVLTree.right, f_pright]
 
 theorem ForallNode.label {a: T} {p: T -> Prop} {left right: AVLTree T}: ForallNode p (AVLNode.mk a left right h) -> p a := by
   intro Hpt
-  cases Hpt with 
+  cases Hpt with
   | some a left right f_pleft f_pa f_pright => exact f_pa
 
 theorem ForallNode.not_mem {a: T} (p: T -> Prop) (t: Option (AVLNode T)): ¬ p a -> ForallNode p t -> a ∉ AVLTree.set t := fun Hnpa Hpt => by
-  cases t with 
+  cases t with
   | none => simp [AVLTree.set]; tauto
   | some t =>
-    cases Hpt with 
+    cases Hpt with
     | some b left right f_pbleft f_pb f_pbright =>
       simp [AVLTree.set_some]
       push_neg
@@ -54,12 +54,12 @@ theorem ForallNode.not_mem {a: T} (p: T -> Prop) (t: Option (AVLNode T)): ¬ p a
       . exact ForallNode.not_mem p left Hnpa f_pbleft
       . exact ForallNode.not_mem p right Hnpa f_pbright
 
-theorem ForallNode.not_mem' {a: T} (p: T -> Prop) (t: Option (AVLNode T)): p a -> ForallNode (fun x =>  ¬p x) t -> a ∉ AVLTree.set t := fun Hpa Hnpt => by 
+theorem ForallNode.not_mem' {a: T} (p: T -> Prop) (t: Option (AVLNode T)): p a -> ForallNode (fun x =>  ¬p x) t -> a ∉ AVLTree.set t := fun Hpa Hnpt => by
   refine' ForallNode.not_mem (fun x => ¬ p x) t _ _
   simp [Hpa]
   exact Hnpt
 
-theorem ForallNode.imp {p q: T -> Prop} {t: AVLTree T}: (∀ x, p x -> q x) -> ForallNode p t -> ForallNode q t := fun Himp Hpt => by 
+theorem ForallNode.imp {p q: T -> Prop} {t: AVLTree T}: (∀ x, p x -> q x) -> ForallNode p t -> ForallNode q t := fun Himp Hpt => by
   induction Hpt
   . simp [ForallNode.none]
   . constructor
@@ -71,24 +71,24 @@ theorem ForallNode.imp {p q: T -> Prop} {t: AVLTree T}: (∀ x, p x -> q x) -> F
 variable [LinearOrder T]
 inductive Invariant: AVLTree T -> Prop
 | none : Invariant none
-| some (a: T) (left: AVLTree T) (right: AVLTree T) : 
+| some (a: T) (left: AVLTree T) (right: AVLTree T) :
   ForallNode (fun v => v < a) left -> ForallNode (fun v => a < v) right
   -> Invariant left -> Invariant right -> Invariant (some (AVLNode.mk a left right h))
 
 @[simp]
 theorem singleton_bst {a: T}: Invariant (some (AVLNode.mk a none none h)) := by
   apply Invariant.some
-  all_goals simp [ForallNode.none, Invariant.none] 
+  all_goals simp [ForallNode.none, Invariant.none]
 
 theorem left {t: AVLTree T}: Invariant t -> Invariant t.left := by
   intro H
-  induction H with 
+  induction H with
   | none => exact Invariant.none
   | some _ _ _ _ _ _ _ _ _ => simp [AVLTree.left]; assumption
 
 theorem right {t: AVLTree T}: Invariant t -> Invariant t.right := by
   intro H
-  induction H with 
+  induction H with
   | none => exact Invariant.none
   | some _ _ _ _ _ _ _ _ _ => simp [AVLTree.right]; assumption
 
@@ -99,16 +99,16 @@ theorem left_pos {left right: Option (AVLNode T)} {a x: T}: BST.Invariant (some 
    . rewrite [Heq] at Hxa; exact absurd Hxa (lt_irrefl _)
    . assumption
    . exfalso
- 
+
      -- Hbst -> x ∈ right -> ForallNode (fun v => ¬ v < a)
      refine' ForallNode.not_mem' (fun v => v < a) right Hxa _ _
      simp [le_of_not_lt]
-     cases Hbst with 
+     cases Hbst with
      | some _ _ _ _ Hforall _ =>
        refine' ForallNode.imp _ Hforall
        exact fun x => le_of_lt
      assumption
- 
+
 theorem right_pos {left right: Option (AVLNode T)} {a x: T}: BST.Invariant (some (AVLNode.mk a left right h)) -> x ∈ AVLTree.set (AVLNode.mk a left right h) -> a < x -> x ∈ AVLTree.set right := fun Hbst Hmem Hax => by
    simp [AVLTree.set_some] at Hmem
    rcases Hmem with (Heq | Hleft) | Hright
@@ -116,12 +116,12 @@ theorem right_pos {left right: Option (AVLNode T)} {a x: T}: BST.Invariant (some
    . exfalso
      refine' ForallNode.not_mem' (fun v => a < v) left Hax _ _
      simp [le_of_not_lt]
-     cases Hbst with 
+     cases Hbst with
      | some _ _ _ Hforall _ _ =>
        refine' ForallNode.imp _ Hforall
        exact fun x => le_of_lt
-     assumption  
+     assumption
    . assumption
- 
+
 
 end BST
