tests/lean/Avl/Rotate.lean
@@ -1,6 +1,5 @@
 import Avl.Tree
 import Avl.AVL
-import Avl.Extracted
 import Avl.Height
 import Avl.BinarySearchTree
 
@@ -9,25 +8,25 @@ namespace Implementation
 open BST (AVLNode.mk')
 open Tree (AVLNode.memoized_height AVLNode.val AVLNode.right AVLNode.left AVLTree.balancingFactor)
 open Primitives
-open avl_verification
+open avl
 
-variable {T: Type} (H: avl_verification.Ord T) [LinearOrder T] (Ospec: OrdSpecLinearOrderEq H)
+variable {T: Type} (H: avl.Ord T) [LinearOrder T] (Ospec: OrdSpecLinearOrderEq H)
 
 @[pspec]
 theorem AVLNode.rotate_right_spec (self: AVLNode T):
-  ∃ rotated t_new, self.rotate_right = .ok (rotated, t_new) 
+  ∃ rotated t_new, self.rotate_right = .ok (rotated, t_new)
   ∧ ((AVLNode.left self).isNone -> rotated = false ∧ t_new = AVLNode.mk (AVLNode.val self) none (AVLNode.right self) (AVLNode.memoized_height self))
   ∧ ∀ self_left, ((AVLNode.left self) = .some self_left -> rotated = true
-    ∧ t_new = 
-      AVLNode.mk' (AVLNode.val self_left) (AVLNode.left self_left) 
+    ∧ t_new =
+      AVLNode.mk' (AVLNode.val self_left) (AVLNode.left self_left)
         (AVLNode.mk' (AVLNode.val self) (AVLNode.right self_left) (AVLNode.right self))
     )
-  := by 
-  match self with 
-  | AVLNode.mk a left right memoized_height => 
-    match left with 
+  := by
+  match self with
+  | AVLNode.mk a left right memoized_height =>
+    match left with
     | .none => simp [AVLNode.rotate_right, AVLNode.left, AVLNode.val, AVLNode.right, AVLNode.memoized_height]
-    | .some (AVLNode.mk b left_left left_right h) => 
+    | .some (AVLNode.mk b left_left left_right h) =>
       simp only [AVLNode.rotate_right, Option.isNone_some, not_false_eq_true, neq_imp, ↓reduceIte,
         core.mem.replace, Option.take, core.mem.swap, Bool.exists_bool]
       right
@@ -44,17 +43,17 @@ theorem AVLNode.rotate_left_spec (self: AVLNode T):
   ∃ rotated t_new, self.rotate_left = .ok (rotated, t_new)
   ∧ ((AVLNode.right self).isNone -> rotated = false ∧ t_new = AVLNode.mk (AVLNode.val self) (AVLNode.left self) none (AVLNode.memoized_height self))
   ∧ ∀ self_right, ((AVLNode.right self) = .some self_right -> rotated = true
-    ∧ t_new = 
-      AVLNode.mk' (AVLNode.val self_right) 
+    ∧ t_new =
+      AVLNode.mk' (AVLNode.val self_right)
         (AVLNode.mk' (AVLNode.val self) (AVLNode.left self) (AVLNode.left self_right))
         (AVLNode.right self_right)
     )
   := by
-  match self with 
-  | AVLNode.mk a left right memoized_height => 
-    match right with 
+  match self with
+  | AVLNode.mk a left right memoized_height =>
+    match right with
     | .none => simp [AVLNode.rotate_left, AVLNode.right, AVLNode.val, AVLNode.left, AVLNode.memoized_height]
-    | .some (AVLNode.mk b right_left right_right h) => 
+    | .some (AVLNode.mk b right_left right_right h) =>
       simp only [AVLNode.rotate_left, Option.isNone_some, not_false_eq_true, neq_imp, ↓reduceIte,
         core.mem.replace, Option.take, core.mem.swap, Bool.exists_bool]
       right
@@ -67,17 +66,17 @@ theorem AVLNode.rotate_left_spec (self: AVLNode T):
       simp [H₂, H₁, AVLNode.val, AVLNode.left]
 
 def AVLNode.rotateLeft (self: AVLNode T): AVLNode T :=
-match self with 
+match self with
 | AVLNode.mk x left right _ =>
-  match right with 
+  match right with
   | none => self
   | some (AVLNode.mk y right_left right_right _) =>
     AVLNode.mk' y (AVLNode.mk' x left right_left) right_right
 
 def AVLNode.rotateRight (self: AVLNode T): AVLNode T :=
-match self with 
+match self with
 | AVLNode.mk x left right _ =>
-  match left with 
+  match left with
   | none => self
   | some (AVLNode.mk y left_left left_right _) =>
     AVLNode.mk' y left_left (AVLNode.mk' x left_right right)
@@ -85,11 +84,11 @@ match self with
 @[pspec]
 lemma AVLNode.rotate_left_spec' (self: AVLNode T):
   ∃ rotated t_new, self.rotate_left = .ok (rotated, t_new)
-  ∧ t_new = AVLNode.rotateLeft self := by 
+  ∧ t_new = AVLNode.rotateLeft self := by
     progress with AVLNode.rotate_left_spec as ⟨ rotated, t_new, Ht ⟩
-    match self with 
+    match self with
     | AVLNode.mk x left right _ =>
-      match right with 
+      match right with
       | none => simp [AVLNode.rotateLeft, Ht, AVLNode.memoized_height]
       | some (AVLNode.mk y right_left right_right _) =>
         simp at Ht; simp [AVLNode.rotateLeft, Ht]
@@ -99,9 +98,9 @@ lemma AVLNode.rotate_right_spec' (self: AVLNode T):
   ∃ rotated t_new, self.rotate_right = .ok (rotated, t_new)
   ∧ t_new = AVLNode.rotateRight self := by
     progress with AVLNode.rotate_right_spec as ⟨ rotated, t_new, Ht ⟩
-    match self with 
+    match self with
     | AVLNode.mk x left right _ =>
-      match left with 
+      match left with
       | none => simp [AVLNode.rotateRight, Ht, AVLNode.memoized_height]
       | some (AVLNode.mk y left_left left_right _) =>
         simp at Ht; simp [AVLNode.rotateRight, Ht]
