tests/lean/Avl/Tree.lean
@@ -1,10 +1,10 @@
-import Avl.Extracted
+import Avl.Funs
+import Avl.Types
 
 namespace Tree
+open avl
 
 variable {T: Type}
-
-open avl_verification
 
 -- Otherwise, Lean cannot prove termination by itself.
 @[reducible]
@@ -60,7 +60,7 @@ def AVLNode.val (t: AVLNode T): T := match t with
 @[simp]
 lemma AVLNode.val_of_mk {x: T} {left right: AVLTree T}: AVLNode.val (AVLNode.mk x left right h) = x := rfl
 
-def AVLNode.memoized_height (t: AVLNode T): Primitives.Scalar .Usize := match t with 
+def AVLNode.memoized_height (t: AVLNode T): Primitives.Scalar .Usize := match t with
 | AVLNode.mk _ _ _ h => h
 
 mutual
@@ -73,7 +73,7 @@ def AVLTree.height: AVLTree T -> Nat
 end
 
 @[simp]
-def AVLTree.height_of_none: @AVLTree.height T none = 0 := rfl
+def AVLTree.height_of_none: @AVLTree.height T none = 0 := by simp [AVLTree.height]
 
 @[simp]
 def AVLTree.height_of_some {t: AVLNode T}: AVLTree.height (some t) = AVLTree.height_node t := by simp [AVLTree.height]
@@ -83,37 +83,37 @@ def AVLTree.height_node_of_mk {left right: AVLTree T}: AVLTree.height_node (AVLN
 
 def AVLTree.height_node_eq (t: AVLNode T): AVLTree.height_node t = 1 + max (AVLTree.height (AVLNode.left t)) (AVLTree.height (AVLNode.right t)) := by sorry
 
-def AVLNode.height_left_lt_tree (left: AVLNode T) {right: AVLTree T}: AVLTree.height_node left < AVLTree.height_node (AVLNode.mk x (some left) right h) := by 
+def AVLNode.height_left_lt_tree (left: AVLNode T) {right: AVLTree T}: AVLTree.height_node left < AVLTree.height_node (AVLNode.mk x (some left) right h) := by
   simp only [AVLTree.height_node_of_mk, AVLTree.height_of_some]
   rw [Nat.add_comm, Nat.add_one]
   exact Nat.lt_succ_of_le (le_max_left _ _)
 
-def AVLNode.height_right_lt_tree (right: AVLNode T) {left: AVLTree T}: AVLTree.height_node right < AVLTree.height_node (AVLNode.mk x left (some right) h) := by 
+def AVLNode.height_right_lt_tree (right: AVLNode T) {left: AVLTree T}: AVLTree.height_node right < AVLTree.height_node (AVLNode.mk x left (some right) h) := by
   simp only [AVLTree.height_node_of_mk, AVLTree.height_of_some]
   rw [Nat.add_comm, Nat.add_one]
   exact Nat.lt_succ_of_le (le_max_right _ _)
 
-def AVLTree.height_left_lt_tree (left right: AVLTree T): AVLTree.height left < AVLTree.height (some (AVLNode.mk x left right h)) := by 
-  match left with 
+def AVLTree.height_left_lt_tree (left right: AVLTree T): AVLTree.height left < AVLTree.height (some (AVLNode.mk x left right h)) := by
+  match left with
   | none => simp [height, height_node]
   | some left => simp only [height, AVLNode.height_left_lt_tree left]
 
-def AVLTree.height_left_lt_tree' (t: AVLNode T): AVLTree.height (AVLNode.left t) < AVLTree.height (some t) := by 
-  match t with 
+def AVLTree.height_left_lt_tree' (t: AVLNode T): AVLTree.height (AVLNode.left t) < AVLTree.height (some t) := by
+  match t with
   | AVLNode.mk _ left right h => simp only [AVLNode.left, AVLTree.height_left_lt_tree]
 
-def AVLTree.height_left_le_tree' (t: AVLTree T): AVLTree.height (AVLTree.left t) ≤ AVLTree.height t := by 
-  match t with 
+def AVLTree.height_left_le_tree' (t: AVLTree T): AVLTree.height (AVLTree.left t) ≤ AVLTree.height t := by
+  match t with
   | none => simp [height, left]
   | some t => simp only [AVLTree.left_of_some, le_of_lt (AVLTree.height_left_lt_tree' t)]
 
-def AVLTree.height_right_lt_tree (left right: AVLTree T): AVLTree.height right < AVLTree.height (some (AVLNode.mk x left right h)) := by 
-  match right with 
+def AVLTree.height_right_lt_tree (left right: AVLTree T): AVLTree.height right < AVLTree.height (some (AVLNode.mk x left right h)) := by
+  match right with
   | none => simp [height, height_node]
   | some right => simp only [height, AVLNode.height_right_lt_tree right]
 
-def AVLTree.height_right_lt_tree' (t: AVLNode T): AVLTree.height (AVLNode.right t) < AVLTree.height (some t) := by 
-  match t with 
+def AVLTree.height_right_lt_tree' (t: AVLNode T): AVLTree.height (AVLNode.right t) < AVLTree.height (some t) := by
+  match t with
   | AVLNode.mk _ left right h => simp only [AVLNode.right, AVLTree.height_right_lt_tree]
 
 
@@ -137,8 +137,11 @@ def AVLTree.mem (tree: AVLTree T) (x: T) :=
   | none => False
   | some (AVLNode.mk y left right _) => x = y ∨ AVLTree.mem left x ∨ AVLTree.mem right x
 
+#check Function.funext_iff
 @[simp]
-def AVLTree.mem_none: AVLTree.mem none = ({}: Set T) := rfl
+def AVLTree.mem_none: AVLTree.mem none = ({}: Set T) := by
+  rw [Function.funext_iff]
+  simp [mem, EmptyCollection.emptyCollection]
 
 @[simp]
 def AVLTree.mem_some {x: T} {left right: AVLTree T}: AVLTree.mem (some (AVLNode.mk x left right h)) = (({x}: Set T) ∪ AVLTree.mem left ∪ AVLTree.mem right) := by
@@ -152,7 +155,7 @@ def AVLTree.mem_some {x: T} {left right: AVLTree T}: AVLTree.mem (some (AVLNode.
 def AVLTree.set (t: AVLTree T): Set T := _root_.setOf (AVLTree.mem t)
 
 @[simp]
-def AVLTree.set_some {x: T} {left right: AVLTree T}: AVLTree.set (some (AVLNode.mk x left right h)) = {x} ∪ AVLTree.set left ∪ AVLTree.set right := by 
+def AVLTree.set_some {x: T} {left right: AVLTree T}: AVLTree.set (some (AVLNode.mk x left right h)) = {x} ∪ AVLTree.set left ∪ AVLTree.set right := by
   simp [set, setOf]
 
 end Tree
